strict_utils.v
@@ -1,0 +1,501 @@
+(* Copyright (c) 2014, Robert Dockins *)
+
+Require Import String.
+Require Import List.
+
+Require Import atoms.
+Require Import permutations.
+
+Require Import basics.
+Require Import preord.
+Require Import categories.
+Require Import sets.
+Require Import finsets.
+Require Import esets.
+Require Import effective.
+Require Import directed.
+Require Import plotkin.
+Require Import joinable.
+Require Import approx_rels.
+Require Import cpo.
+Require Import profinite.
+Require Import profinite_adj.
+
+
+Notation up f := (L@(U@f) ∘ adj_counit_inv_hom _) (only parsing).
+Notation pi1 := PLT.pi1.
+Notation pi2 := PLT.pi2.
+Notation ε := (adj_counit _).
+Notation η := (adj_unit _).
+Notation γ := (adj_counit_inv_hom _).
+Arguments PLT.pair_map [hf] [A B C D] f g.
+Notation "A × B" := (@PLT.prod false A B).
+Notation "A ⊗ B" := (@PLT.prod true A B)
+   (at level 54, right associativity).
+Notation "A ⊸ B" := (@PLT.exp true A B)
+   (at level 50, left associativity).
+Notation "A ⇒ B" := (@PLT.exp false A B).
+
+Definition lift (X:PLT) : PLT := U (L X).
+Definition colift (X:∂PLT) : ∂PLT := L (U X).
+
+Definition strict_app (A B:∂PLT) 
+  : U (A ⊸ B) × U A → U B
+
+  := U@( @PLT.app _ A B ∘ PLT.pair_map ε ε ∘ lift_prod' _ _) ∘ η.
+
+Definition strict_curry (Γ:PLT) (A B:∂PLT)
+  (f:Γ×U A → U B) : Γ → U (A ⊸ B) 
+
+  := U@( PLT.curry( ε ∘ L@f ∘ lift_prod _ _ ∘ PLT.pair_map id γ) ) ∘ η.
+  
+Definition strict_app' (A B:∂PLT) 
+  : U (colift (A ⊸ B)) × U A → U B 
+
+  := strict_app A B ∘ PLT.pair_map (U@ε) id.
+
+Definition strict_curry' (Γ:PLT) (A B:∂PLT)
+  (f:Γ × U A → U B) : Γ → U (colift (A ⊸ B))
+
+  := η ∘ strict_curry Γ A B f.
+
+Transparent liftPPLT.
+Lemma hom_rel_U (A B:∂PLT) (f:A → B) (a:U A) (b:U B) :
+  (a,b) ∈ PLT.hom_rel (U@f) <->
+  (b = None \/ exists a' b', (a',b') ∈ PLT.hom_rel f /\ a = Some a' /\ b = Some b').
+Proof.
+  simpl. split; intros.
+  rewrite  (liftPPLT_rel_elem _ _ _ _ a b) in H.
+  destruct H.
+  destruct b; auto.
+  destruct H. elim H.
+  destruct H as [p [q [?[??]]]].
+  right.
+  destruct a.
+  destruct b.
+  exists c. exists c0. split; auto.
+  revert H. apply PLT.hom_order; auto.
+  destruct H1. elim H2.
+  destruct H0. elim H2.
+  apply liftPPLT_rel_elem.
+  destruct H. subst b; auto.
+  destruct H as [p [q [?[??]]]].
+  subst a b.
+  right.   eauto.
+Qed.
+Opaque liftPPLT.
+
+Lemma hom_rel_L (A B:PLT) (f:A → B) (a:L A) (b:L B) :
+  (a,b) ∈ PLT.hom_rel (L@f) <-> (a,b) ∈ PLT.hom_rel f.
+Proof.
+  split; auto.
+Qed.
+
+
+Definition semvalue (Γ:PLT) (A:∂PLT) (f:Γ → U A) :=
+  forall g, exists a, (g,Some a) ∈ PLT.hom_rel f.
+Arguments semvalue [Γ A] f.
+
+Lemma strict_curry_app2 D (Γ:PLT) (A B:∂PLT) 
+  (f : Γ×U A → U B) (g : D → U A) (h:D → Γ) (Hg : semvalue g) :
+
+  strict_app A B ∘ PLT.pair (strict_curry Γ A B f ∘ h) g ≈ f ∘ PLT.pair h g.
+Proof.
+  unfold strict_app, strict_curry.
+  simpl.
+  rewrite <- (cat_assoc PLT).
+  rewrite (NT.axiom adj_unit
+    (PLT.pair
+          (U @
+           PLT.curry
+             (adj_counit_hom B ∘ L @ f ∘ lift_prod Γ (U A)
+              ∘ PLT.pair_map id γ) ∘ adj_unit_hom Γ ∘ h) g)).
+  simpl.
+  rewrite (cat_assoc PLT).
+  rewrite <- (Functor.compose U). 2: reflexivity.
+  rewrite <- (cat_assoc ∂PLT).
+  rewrite <- lift_prod_pair'.
+  rewrite <- (cat_assoc ∂PLT).
+  rewrite <- (PLT.pair_map_pair true).
+  rewrite (Functor.compose L). 2: reflexivity.
+  rewrite <- (cat_assoc ∂PLT).
+  rewrite <- (cat_assoc ∂PLT).
+  generalize (NT.axiom adj_counit
+    (PLT.curry (adj_counit_hom B
+                ∘ (L @ f ∘ (lift_prod Γ (U A) ∘ PLT.pair_map id γ))))).
+  simpl; intros.
+  etransitivity.
+  apply cat_respects. 2: reflexivity.
+  apply (Functor.respects U).
+  apply cat_respects. reflexivity.
+  apply PLT.pair_eq. 2: reflexivity.
+  rewrite (cat_assoc ∂PLT).
+  rewrite (Functor.compose L). 2: reflexivity.
+  rewrite (cat_assoc ∂PLT).
+  apply cat_respects. 2: reflexivity.
+  apply cat_respects. 2: reflexivity.
+  apply H. clear H.
+  rewrite <- (cat_assoc ∂PLT).
+  rewrite <- (cat_assoc ∂PLT).
+  generalize (Adjunction.adjoint_axiom1 PLT_adjoint Γ).
+  simpl. intros. 
+  rewrite (cat_assoc ∂PLT _ _ _ _
+    (adj_counit_hom (L Γ))).
+  rewrite H. clear H.
+  rewrite (cat_ident2 ∂PLT).
+  rewrite (PLT.curry_apply3 true).
+  repeat rewrite <- (cat_assoc ∂PLT).
+  rewrite <- (PLT.pair_map_pair true).
+  assert (PLT.pair (id ∘ L@h)
+             (adj_counit_inv_hom A ∘ (adj_counit_hom A ∘ forgetPLT @ g)) 
+             ≈
+          PLT.pair (L@h) (L@g)).
+  apply PLT.pair_eq.
+  apply cat_ident2.
+  rewrite (cat_assoc ∂PLT).
+  apply adj_inv_eq. auto.
+  etransitivity.
+  apply cat_respects. 2: reflexivity.
+  apply Functor.respects.
+  apply cat_respects. reflexivity.
+  apply cat_respects. reflexivity.
+  apply cat_respects. reflexivity. apply H.
+  rewrite lift_prod_pair.
+  rewrite <- (Functor.compose L). 2: reflexivity.
+  rewrite (Functor.compose U). 2: reflexivity.
+  rewrite <- (cat_assoc PLT).
+  rewrite <- (NT.axiom adj_unit (f ∘ PLT.pair h g)). simpl.
+  rewrite (cat_assoc PLT).
+  generalize (Adjunction.adjoint_axiom2 PLT_adjoint B).
+  simpl. intros. rewrite H0.
+  apply cat_ident2.
+Qed.  
+
+
+Lemma strict_curry_app (Γ:PLT) (A B:∂PLT) 
+  (f : Γ×U A → U B) (g : Γ → U A) (Hg: semvalue g) :
+  strict_app A B ∘ PLT.pair (strict_curry Γ A B f) g ≈ f ∘ PLT.pair id g.
+Proof.
+  generalize (strict_curry_app2 Γ Γ A B f g id Hg).
+  rewrite (cat_ident1 PLT). auto.
+Qed.
+
+Lemma strict_curry_app2' D (Γ:PLT) (A B:∂PLT) 
+  (f : Γ×U A → U B) (g : D → U A) (h:D → Γ) (Hg : semvalue g) :
+
+  strict_app' A B ∘ PLT.pair (strict_curry' Γ A B f ∘ h) g ≈ f ∘ PLT.pair h g.
+Proof.
+  unfold strict_curry'.
+  unfold strict_app'.
+  rewrite <- (cat_assoc PLT).
+  rewrite <- (PLT.pair_map_pair false).
+  rewrite (cat_assoc PLT).
+  rewrite (cat_assoc PLT).
+  rewrite (cat_ident2 PLT).
+  generalize (Adjunction.adjoint_axiom2 PLT_adjoint (A ⊸ B)).
+  intros. simpl in H. rewrite H.
+  rewrite (cat_ident2 PLT).
+  apply strict_curry_app2. auto.
+Qed.
+
+Lemma strict_curry_app' (Γ:PLT) (A B:∂PLT) 
+  (f : Γ×U A → U B) (g : Γ → U A) (Hg : semvalue g) :
+
+  strict_app' A B ∘ PLT.pair (strict_curry' Γ A B f) g ≈ f ∘ PLT.pair id g.
+Proof.
+  generalize (strict_curry_app2' Γ Γ A B f g id Hg).
+  rewrite (cat_ident1 PLT). auto.
+Qed.
+
+
+Lemma plt_strict_compose : forall (A B C:∂PLT) (f:B → C),
+  f ∘ (⊥: A → B) ≈ ⊥.
+Proof.
+  intros. split. 2: apply bottom_least.
+  hnf. intros.
+  destruct a. apply compose_hom_rel in H.
+  destruct H as [y [??]].
+  simpl in H.
+  apply union_axiom in H. destruct H as [X[??]].
+  apply image_axiom2 in H. destruct H as [q [??]].
+  apply empty_elem in H. elim H.
+Qed.
+
+
+Lemma strict_app_bot (Γ:PLT) (A B:∂PLT) (f:Γ → U (A ⊸ B)) :
+  strict_app A B ∘ PLT.pair f ⊥ ≈ ⊥.
+Proof.
+  unfold strict_app. simpl.
+  rewrite <- (cat_assoc PLT).
+
+  generalize (NT.axiom adj_unit). simpl; intros.
+  rewrite H.
+  rewrite (cat_assoc PLT).
+  rewrite <- (Functor.compose U). 2: reflexivity.
+  rewrite <- (cat_assoc ∂PLT).
+  rewrite <- lift_prod_pair'.
+  rewrite <- (cat_assoc ∂PLT).
+  rewrite <- (PLT.pair_map_pair true).
+  etransitivity.
+  apply cat_respects. 2: reflexivity.
+  apply Functor.respects.
+  etransitivity.
+  apply cat_respects. reflexivity.
+  2: apply plt_strict_compose.
+  etransitivity.
+  apply PLT.pair_eq. reflexivity.
+  2: apply PPLT.pair_bot1.
+  generalize (NT.axiom adj_counit). simpl; intros.
+  rewrite (Functor.compose L). 2: reflexivity.
+  rewrite (cat_assoc ∂PLT).
+  rewrite H0. 
+  rewrite <- (cat_assoc ∂PLT).
+  generalize (Adjunction.adjoint_axiom1 PLT_adjoint Γ).
+  intros. simpl in H1. rewrite H1.
+  apply cat_ident1.
+  auto.
+Qed.
+
+Lemma strict_app_bot' (Γ:PLT) (A B:∂PLT) (f:Γ → U (colift (A ⊸ B))) :
+  strict_app' A B ∘ PLT.pair f ⊥ ≈ ⊥.
+Proof.
+  unfold strict_app'.
+  rewrite <- (cat_assoc PLT).
+  rewrite <- (PLT.pair_map_pair false).
+  rewrite (cat_ident2 PLT).
+  apply strict_app_bot.
+Qed.
+
+Section fixes.
+  Variable Γ:PLT.
+  Variable A:∂PLT.
+  Variable f:Γ → U A ⇒ U A.
+
+  Definition fixes_step
+    (x:Γ → U A) : Γ → U A :=
+
+    PLT.app ∘ PLT.pair f x.
+
+  Program Definition fixes_step' : PLT.homset_cpo _ Γ (U A) → PLT.homset_cpo _ Γ (U A) :=
+    CPO.Hom _ (PLT.homset_cpo _ Γ (U A)) (PLT.homset_cpo _ Γ (U A)) fixes_step _ _.
+  Next Obligation.
+    intros. unfold fixes_step.
+    apply PLT.compose_mono; auto.
+    apply PLT.pair_monotone; auto.
+  Qed.    
+  Next Obligation.
+  Admitted.
+
+  Definition fixes : Γ → U A := lfp fixes_step'.
+
+  Lemma fixes_unroll :
+    fixes ≈ PLT.app ∘ PLT.pair f fixes.
+  Proof.
+    unfold fixes at 1.
+    rewrite <- lfp_fixpoint. simpl. unfold fixes_step.
+    auto.
+  Qed.
+
+End fixes.
+
+Arguments strict_app [A B].
+Arguments strict_curry [Γ A B] f.
+
+Arguments strict_app' [A B].
+Arguments strict_curry' [Γ A B] f.
+
+
+
+Lemma semvalue_le : forall Γ A (f f':Γ → U A),
+  f ≤ f' -> semvalue f -> semvalue f'.
+Proof.
+  repeat intro.
+  destruct (H0 g). exists x.
+  apply H. auto.
+Qed.
+
+Lemma semvalue_equiv : forall Γ A (f f':Γ → U A),
+  f ≈ f' -> semvalue f -> semvalue f'.
+Proof.
+  intros Γ A f f' H. apply semvalue_le; auto.
+Qed.
+
+Require Import Setoid.
+
+Add Parametric Morphism Γ A :
+  (@semvalue Γ A)
+  with signature (eq_op _) ==> iff
+    as semvalue_eq_morphism.
+Proof.
+  intros. split; apply semvalue_equiv; auto.
+Qed.
+
+Lemma eta_semvalue A B (f:A → B) :
+  semvalue (η ∘ f).
+Proof.
+  repeat intro.
+  destruct (PLT.hom_directed _ _ _ f g nil). hnf; auto.
+  hnf. intros. apply nil_elem in H. elim H.
+  destruct H. apply erel_image_elem in H0.
+  exists x. 
+  simpl NT.transform.
+  simpl. apply compose_elem.
+  apply PLT.hom_order.
+  exists x. split; auto.
+  apply adj_unit_rel_elem. auto.
+Qed.
+
+Lemma strict_curry'_semvalue Γ A B f :
+  semvalue (@strict_curry' Γ A B f).
+Proof.
+  unfold strict_curry'.
+  apply eta_semvalue.  
+Qed.
+
+Lemma strict_curry'_semvalue2 Γ A B C f (g:C → Γ) :
+  semvalue (@strict_curry' Γ A B f ∘ g).
+Proof.
+  unfold strict_curry'.
+  rewrite <- (cat_assoc PLT).
+  apply eta_semvalue.  
+Qed.
+
+
+Lemma hom_rel_pair hf (A B C:PLT.PLT hf) (f:C → A) (g:C → B) c x y :
+  (c,(x,y)) ∈ PLT.hom_rel (PLT.pair f g) <->
+  ((c,x) ∈ PLT.hom_rel f /\ (c,y) ∈ PLT.hom_rel g).
+Proof.
+  simpl; split; intros.
+  apply pair_rel_elem in H. auto.
+  apply pair_rel_elem; auto.
+Qed.
+
+Lemma hom_rel_pair_map hf (A B C D:PLT.PLT hf) (f:A → C) (g:B → D) x y x' y' :
+  (x,y,(x',y')) ∈ PLT.hom_rel (PLT.pair_map f g) <->
+  ((x,x') ∈ PLT.hom_rel f /\ (y,y') ∈ PLT.hom_rel g).
+Proof.
+  unfold PLT.pair_map.
+  split; intros.
+  rewrite (hom_rel_pair _ _ _ _ (f∘pi1) (g∘pi2) (x,y) x' y') in H.
+  destruct H.
+  apply compose_hom_rel in H.
+  destruct H as [?[??]].
+  apply compose_hom_rel in H0.
+  destruct H0 as [?[??]].
+  simpl in H. 
+  rewrite (pi1_rel_elem _ _ _ _ x y x0)  in H.
+  simpl in H0.
+  rewrite (pi2_rel_elem _ _ _ _ x y x1) in H0.
+  split.
+  revert H1. apply PLT.hom_order; auto.
+  revert H2. apply PLT.hom_order; auto.
+  rewrite (hom_rel_pair _ _ _ _ (f∘pi1) (g∘pi2)).
+  destruct H.
+  split.
+  apply compose_hom_rel.
+  exists x. split; auto. simpl. apply pi1_rel_elem; auto.
+  apply compose_hom_rel.
+  exists y. split; auto. simpl. apply pi2_rel_elem; auto.
+Qed.
+
+Lemma semvalue_strict_app_out1 A B C (f:C → U (A ⊸ B)) (x:C → U A) :
+  semvalue (strict_app ∘ PLT.pair f x) ->
+  semvalue f.
+Proof.
+  intros. red; intro.
+  destruct (H g) as [a ?].
+  rewrite (compose_hom_rel false _ _ _ _ strict_app g (Some a)) in H0.
+  destruct H0 as [[f' x'] [??]].
+  rewrite (hom_rel_pair _ _ _ _ f x) in H0.
+  destruct H0.
+  unfold strict_app in H1.
+  rewrite (compose_hom_rel false _ _ _ η 
+    (U@(PLT.app ∘ PLT.pair_map ε ε ∘ lift_prod' (U (A ⊸ B)) (U A)))) in H1.
+  destruct H1 as [q [??]].
+  simpl in H1.
+  apply adj_unit_rel_elem in H1.
+  rewrite (hom_rel_U _ _ _ q (Some a)) in H3.
+  destruct H3. discriminate.
+  destruct H3 as [p' [q' [?[??]]]]. subst q. inversion H5; subst.
+  apply compose_hom_rel in H3.
+  destruct H3 as [[??][??]].
+  simpl in H3. apply ident_elem in H3.
+  apply compose_hom_rel in H4.
+  destruct H4 as [[??][??]].
+  rewrite (hom_rel_pair_map _ _ _ _ _ _ _ c c0 c1 c2) in H4.
+  destruct H4.
+  simpl in H4. apply adj_counit_rel_elem in H4.
+  destruct c. 2: elim H4.
+  destruct H1. simpl in H1.
+  destruct H3. simpl in H3.
+  rewrite <- H3 in H1. destruct f'.
+  exists c3. auto.
+  elim H1.
+Qed.
+
+Lemma semvalue_strict_app_out2 A B C (f:C → U (A ⊸ B)) (x:C → U A) :
+  semvalue (strict_app ∘ PLT.pair f x) ->
+  semvalue x.
+Proof.
+  intros. red; intro.
+  destruct (H g) as [a ?].
+  rewrite (compose_hom_rel false _ _ _ _ strict_app g (Some a)) in H0.
+  destruct H0 as [[f' x'] [??]].
+  rewrite (hom_rel_pair _ _ _ _ f x) in H0.
+  destruct H0.
+  unfold strict_app in H1.
+  rewrite (compose_hom_rel false _ _ _ η 
+    (U@(PLT.app ∘ PLT.pair_map ε ε ∘ lift_prod' (U (A ⊸ B)) (U A)))) in H1.
+  destruct H1 as [q [??]].
+  simpl in H1.
+  apply adj_unit_rel_elem in H1.
+  rewrite (hom_rel_U _ _ _ q (Some a)) in H3.
+  destruct H3. discriminate.
+  destruct H3 as [p' [q' [?[??]]]]. subst q. inversion H5; subst.
+  apply compose_hom_rel in H3.
+  destruct H3 as [[??][??]].
+  simpl in H3. apply ident_elem in H3.
+  apply compose_hom_rel in H4.
+  destruct H4 as [[??][??]].
+  rewrite (hom_rel_pair_map _ _ _ _ _ _ _ c c0 c1 c2) in H4.
+  destruct H4.
+  simpl in H7. apply adj_counit_rel_elem in H7.
+  destruct c0. 2: elim H7.
+  destruct H1. simpl in H1.
+  destruct H3. simpl in H3.
+  rewrite <- H9 in H8. simpl in H8.
+  destruct x'. exists c3. auto.
+  elim H8.
+Qed.
+
+Lemma semvalue_app_out1' A B C (f:C → U (colift (A ⊸ B))) (x:C → U A) :
+  semvalue (strict_app' ∘ PLT.pair f x) ->
+  semvalue f.
+Proof.
+  intros.
+  unfold strict_app' in H.
+  rewrite <- (cat_assoc PLT) in H.
+  rewrite <- (PLT.pair_map_pair false) in H.
+  apply semvalue_strict_app_out1 in H.
+  red; intros.
+  destruct (H g) as [a ?].
+  rewrite (compose_hom_rel _ _ _ _ f (U@ε) g (Some a)) in H0.
+  destruct H0 as [q [??]].
+  rewrite (hom_rel_U _ _ _ q (Some a)) in H1.
+  destruct H1. discriminate.
+  destruct H1 as [?[?[?[??]]]]. subst.
+  exists x0. auto.
+Qed.
+
+Lemma semvalue_app_out2' A B C (f:C → U (colift (A ⊸ B))) (x:C → U A) :
+  semvalue (strict_app' ∘ PLT.pair f x) ->
+  semvalue x.
+Proof.
+  intros.
+  unfold strict_app' in H.
+  rewrite <- (cat_assoc PLT) in H.
+  rewrite <- (PLT.pair_map_pair false) in H.
+  apply semvalue_strict_app_out2 in H.
+  rewrite (cat_ident2 PLT) in H. auto.
+Qed.
+
